<?xml version="1.0"?>


<!DOCTYPE rdf:RDF [
    <!ENTITY owl "http://www.w3.org/2002/07/owl#" >
    <!ENTITY xsd "http://www.w3.org/2001/XMLSchema#" >
    <!ENTITY owl2xml "http://www.w3.org/2006/12/owl2-xml#" >
    <!ENTITY rdfs "http://www.w3.org/2000/01/rdf-schema#" >
    <!ENTITY rdf "http://www.w3.org/1999/02/22-rdf-syntax-ns#" >
    <!ENTITY cpannotationschema "http://www.ontologydesignpatterns.org/schemas/cpannotationschema.owl#" >
]>


<rdf:RDF xmlns="http://semantic.cs.put.poznan.pl/ontologies/newsreportingevent.owl#"
     xml:base="http://semantic.cs.put.poznan.pl/ontologies/newsreportingevent.owl"
     xmlns:rdf="http://www.w3.org/1999/02/22-rdf-syntax-ns#"
     xmlns:owl="http://www.w3.org/2002/07/owl#"
     xmlns:owl2xml="http://www.w3.org/2006/12/owl2-xml#"
     xmlns:cpannotationschema="http://www.ontologydesignpatterns.org/schemas/cpannotationschema.owl#"
     xmlns:xsd="http://www.w3.org/2001/XMLSchema#"
     xmlns:rdfs="http://www.w3.org/2000/01/rdf-schema#">
    <owl:Ontology rdf:about="http://semantic.cs.put.poznan.pl/ontologies/newsreportingevent.owl">
        <cpannotationschema:hasComponent>http://ontologydesignpatterns.org/wiki/Submissions:IntensionExtension</cpannotationschema:hasComponent>
        <cpannotationschema:coversRequirements xml:lang="en">
In addition to the competency questions defined for pattern
ReportingEvent (http:/ontologydesignpatterns.org/wiki/Submissions:ReportingEvent)
the pattern allows to answer the following questions:
- What aspects of an actual event were presented in the news message?
- Who reported an actual event? Which news provider they represented?
- When was a certain actual event reported for the first time?
- What actual events are presented in a certain medium/by media of a certain news provider?
- How was an actual event presented?
		</cpannotationschema:coversRequirements>
        <cpannotationschema:hasComponent>http://ontologydesignpatterns.org/wiki/Submissions:Types_of_entities</cpannotationschema:hasComponent>
        <cpannotationschema:hasComponent>http://ontologydesignpatterns.org/wiki/Submissions:ReportingEvent</cpannotationschema:hasComponent>
        <cpannotationschema:hasComponent>http://ontologydesignpatterns.org/wiki/Submissions:ActingFor</cpannotationschema:hasComponent>
        <cpannotationschema:hasComponent>http://ontologydesignpatterns.org/wiki/Submissions:TimeIndexedSituation</cpannotationschema:hasComponent>
        <cpannotationschema:scenarios xml:lang="en">
A single actual event, bus drivers protest, is presented in to different media: a TV news station
and a news website. John Doe prepared the material for the station Channel 55, owned by Media Corp.
This material was presented as first material in a news programme on 16/07/2016, started at 19:30 and ended at 19:35.
It was based on correspondent report. The material said that the cause of the protest was malfunction of buses,
and that a brutal police intervention took place.

The article from website livingintheworld.com also mentioned malfunction of buses, but it also mentioned
other cause of protest: planned reduction of social benefits. It did not mention brutal police intervention,
but it did mention destruction of public property. The article seems not important for the website authors,
it was presented at the page bottom.
		</cpannotationschema:scenarios>
        <cpannotationschema:relatedCPs xml:lang="en">
Pattern NewsReportingEvent is an extension of ReportingEvent pattern.

Pattern ActingFor (http:/ontologydesignpatterns.org/wiki/Submissions:ActingFor) is a component of this pattern.
It allows to model the fact that NewsEventReporter (Agent) acts for NewsProvider (SocialAgent).

TODO describe time indexed situation
		</cpannotationschema:relatedCPs>
        <cpannotationschema:hasIntent xml:lang="en">
The pattern can be used for modelling situations
in which we are not certain that a particular actual event has the properties
which were described in a news message. We want to define the properties
of an actual event which were reported (time, place, actors, subevents,
cause, effect etc.), but not to treat them as universal, verified knowledge.
The pattern also allows to define who is responsible for a particular
description of an event and how this description is dealt with.
		</cpannotationschema:hasIntent>
        <cpannotationschema:hasConsequences xml:lang="en">
The pattern is rather complex and should only be used if the circumstances of the events presented in a media
are expected to be uncertain (to differ in different news event reports of different news providers).
		</cpannotationschema:hasConsequences>
        <rdfs:comment xml:lang="en">Pattern description is available at: http://ontologydesignpatterns.org/wiki/Submissions:NewsReportingEvent</rdfs:comment>
        <rdfs:comment xml:lang="en">Pattern description is included in: E. Kowalczuk, A. ≈Åawrynowicz, &quot;The Reporting Event Ontology Design Pattern and Its Extension to Report News Events&quot; (2016).</rdfs:comment>
        <rdfs:comment xml:lang="en">This ontology is a formalisation of the News Reporting Event ontology design pattern.</rdfs:comment>
        <owl:imports rdf:resource="http://semantic.cs.put.poznan.pl/ontologies/reportingevent.owl"/>
        <owl:imports rdf:resource="http://www.ontologydesignpatterns.org/cp/owl/actingfor.owl"/>
        <owl:imports rdf:resource="http://www.ontologydesignpatterns.org/cp/owl/timeindexedsituation.owl"/>
    </owl:Ontology>
    


    <!-- 
    ///////////////////////////////////////////////////////////////////////////////////////
    //
    // Object Properties
    //
    ///////////////////////////////////////////////////////////////////////////////////////
     -->

    


    <!-- http://semantic.cs.put.poznan.pl/ontologies/newsreportingevent.owl#hasPresentationContext -->

    <owl:ObjectProperty rdf:about="http://semantic.cs.put.poznan.pl/ontologies/newsreportingevent.owl#hasPresentationContext">
        <rdfs:comment xml:lang="en">This property can be used to link NewsReportingEvent to a NewsPresentationContext.</rdfs:comment>
        <rdfs:range rdf:resource="http://semantic.cs.put.poznan.pl/ontologies/newsreportingevent.owl#PresentationContext"/>
        <rdfs:subPropertyOf rdf:resource="http://www.ontologydesignpatterns.org/cp/owl/situation.owl#isSettingFor"/>
    </owl:ObjectProperty>
    


    <!-- http://semantic.cs.put.poznan.pl/ontologies/newsreportingevent.owl#owns -->

    <owl:ObjectProperty rdf:about="http://semantic.cs.put.poznan.pl/ontologies/newsreportingevent.owl#owns">
        <rdfs:comment xml:lang="en">This property can be used to link a certain NewsProvider with a Media that the NewsProvider ows, e.g. Fox News Channel is owned by Fox Entertainment Group, which also owns other Media (FXX Channel, etc.).
This is an universal property, it can be also used in different context (e.g. Ruslana owns a Persian cat).</rdfs:comment>
    </owl:ObjectProperty>
    


    <!-- http://semantic.cs.put.poznan.pl/ontologies/newsreportingevent.owl#presentedAt -->

    <owl:ObjectProperty rdf:about="http://semantic.cs.put.poznan.pl/ontologies/newsreportingevent.owl#presentedAt">
        <rdfs:comment xml:lang="en">This property can be used to link a NewsReportingEvent to a Media (TV station, radio station, newspaper, webpage) at which a certain ActualEventView was presented. 
This is an universal property and can be used in different contexts.</rdfs:comment>
    </owl:ObjectProperty>
    


    <!-- http://semantic.cs.put.poznan.pl/ontologies/reportingevent.owl#reports -->

    <rdf:Description rdf:about="http://semantic.cs.put.poznan.pl/ontologies/reportingevent.owl#reports">
        <rdfs:subPropertyOf rdf:resource="http://www.ontologydesignpatterns.org/cp/owl/timeindexedsituation.owl#forEntity"/>
    </rdf:Description>
    


    <!-- 
    ///////////////////////////////////////////////////////////////////////////////////////
    //
    // Classes
    //
    ///////////////////////////////////////////////////////////////////////////////////////
     -->

    


    <!-- http://semantic.cs.put.poznan.pl/ontologies/newsreportingevent.owl#Media -->

    <owl:Class rdf:about="http://semantic.cs.put.poznan.pl/ontologies/newsreportingevent.owl#Media">
        <rdfs:subClassOf rdf:resource="http://www.ontologydesignpatterns.org/cp/owl/typesofentities.owl#Object"/>
        <rdfs:subClassOf>
            <owl:Restriction>
                <owl:onProperty>
                    <rdf:Description>
                        <owl:inverseOf rdf:resource="http://semantic.cs.put.poznan.pl/ontologies/newsreportingevent.owl#owns"/>
                    </rdf:Description>
                </owl:onProperty>
                <owl:onClass rdf:resource="http://semantic.cs.put.poznan.pl/ontologies/newsreportingevent.owl#NewsProvider"/>
                <owl:qualifiedCardinality rdf:datatype="&xsd;nonNegativeInteger">1</owl:qualifiedCardinality>
            </owl:Restriction>
        </rdfs:subClassOf>
        <rdfs:comment xml:lang="en">An entity that allows a communication of news messages, for example a TV station, radio station, newspaper, website, etc.</rdfs:comment>
    </owl:Class>
    


    <!-- http://semantic.cs.put.poznan.pl/ontologies/newsreportingevent.owl#NewsEventReporter -->

    <owl:Class rdf:about="http://semantic.cs.put.poznan.pl/ontologies/newsreportingevent.owl#NewsEventReporter">
        <rdfs:subClassOf rdf:resource="http://semantic.cs.put.poznan.pl/ontologies/reportingevent.owl#EventReporter"/>
        <rdfs:subClassOf rdf:resource="http://www.ontologydesignpatterns.org/cp/owl/actingfor.owl#Agent"/>
        <rdfs:subClassOf>
            <owl:Restriction>
                <owl:onProperty>
                    <rdf:Description>
                        <owl:inverseOf rdf:resource="http://semantic.cs.put.poznan.pl/ontologies/reportingevent.owl#hasAuthor"/>
                    </rdf:Description>
                </owl:onProperty>
                <owl:someValuesFrom rdf:resource="http://semantic.cs.put.poznan.pl/ontologies/newsreportingevent.owl#NewsReportingEvent"/>
            </owl:Restriction>
        </rdfs:subClassOf>
        <rdfs:comment xml:lang="en">An Actor (usually a Person) that is an author of a certain ActualEventView.
NewsEventReporter is not linked to an ActualEventView directly, it is connected to NewsReportingEvent, which is designed to document the act of reporting.</rdfs:comment>
    </owl:Class>
    


    <!-- http://semantic.cs.put.poznan.pl/ontologies/newsreportingevent.owl#NewsPresentationContext -->

    <owl:Class rdf:about="http://semantic.cs.put.poznan.pl/ontologies/newsreportingevent.owl#NewsPresentationContext">
        <rdfs:subClassOf rdf:resource="http://semantic.cs.put.poznan.pl/ontologies/newsreportingevent.owl#PresentationContext"/>
        <rdfs:subClassOf>
            <owl:Restriction>
                <owl:onProperty>
                    <rdf:Description>
                        <owl:inverseOf rdf:resource="http://semantic.cs.put.poznan.pl/ontologies/newsreportingevent.owl#hasPresentationContext"/>
                    </rdf:Description>
                </owl:onProperty>
                <owl:someValuesFrom rdf:resource="http://semantic.cs.put.poznan.pl/ontologies/newsreportingevent.owl#NewsReportingEvent"/>
            </owl:Restriction>
        </rdfs:subClassOf>
        <rdfs:comment xml:lang="en">Class for denoting circumstances of an actual event presentation. For example if an event was presented at the end of website, then end of website is its NewsPresentationContext.
NewsPresentationContext is not directly attached to an ActualEventView, it is attached to NewsReportingEvent, which designates the act of an event reporting.</rdfs:comment>
    </owl:Class>
    


    <!-- http://semantic.cs.put.poznan.pl/ontologies/newsreportingevent.owl#NewsProvider -->

    <owl:Class rdf:about="http://semantic.cs.put.poznan.pl/ontologies/newsreportingevent.owl#NewsProvider">
        <rdfs:subClassOf rdf:resource="http://www.ontologydesignpatterns.org/cp/owl/actingfor.owl#SocialAgent"/>
        <rdfs:subClassOf>
            <owl:Restriction>
                <owl:onProperty rdf:resource="http://semantic.cs.put.poznan.pl/ontologies/newsreportingevent.owl#owns"/>
                <owl:someValuesFrom rdf:resource="http://semantic.cs.put.poznan.pl/ontologies/newsreportingevent.owl#Media"/>
            </owl:Restriction>
        </rdfs:subClassOf>
        <rdfs:comment xml:lang="en">An entity, usually a company, that ows a certain Media. For example Fox Entertainment Group owns the Fox News Channel. Fox Entertainment Group is a NewsProvider.</rdfs:comment>
    </owl:Class>
    


    <!-- http://semantic.cs.put.poznan.pl/ontologies/newsreportingevent.owl#NewsReportingEvent -->

    <owl:Class rdf:about="http://semantic.cs.put.poznan.pl/ontologies/newsreportingevent.owl#NewsReportingEvent">
        <rdfs:subClassOf rdf:resource="http://semantic.cs.put.poznan.pl/ontologies/reportingevent.owl#ReportingEvent"/>
        <rdfs:subClassOf rdf:resource="http://www.ontologydesignpatterns.org/cp/owl/timeindexedsituation.owl#TimeIndexedSituation"/>
        <rdfs:subClassOf>
            <owl:Restriction>
                <owl:onProperty rdf:resource="http://semantic.cs.put.poznan.pl/ontologies/newsreportingevent.owl#presentedAt"/>
                <owl:someValuesFrom rdf:resource="http://semantic.cs.put.poznan.pl/ontologies/newsreportingevent.owl#Media"/>
            </owl:Restriction>
        </rdfs:subClassOf>
        <rdfs:subClassOf>
            <owl:Restriction>
                <owl:onProperty rdf:resource="http://semantic.cs.put.poznan.pl/ontologies/reportingevent.owl#hasAuthor"/>
                <owl:someValuesFrom rdf:resource="http://semantic.cs.put.poznan.pl/ontologies/newsreportingevent.owl#NewsEventReporter"/>
            </owl:Restriction>
        </rdfs:subClassOf>
        <rdfs:comment xml:lang="en">This is a subclass of ReportingEvent, designed to represent an act of reporting a certain actual event during a news programme or via other news media.</rdfs:comment>
    </owl:Class>
    


    <!-- http://semantic.cs.put.poznan.pl/ontologies/newsreportingevent.owl#PresentationContext -->

    <owl:Class rdf:about="http://semantic.cs.put.poznan.pl/ontologies/newsreportingevent.owl#PresentationContext">
        <rdfs:subClassOf rdf:resource="http://www.ontologydesignpatterns.org/cp/owl/typesofentities.owl#Entity"/>
        <rdfs:comment xml:lang="en">Class for denoting circumstances of an entity presentation. If a waiter presented a dish with an apologetic smile, then the apologetic smile is a PresentationContext.</rdfs:comment>
    </owl:Class>
</rdf:RDF>



<!-- Generated by the OWL API (version 3.5.0) http://owlapi.sourceforge.net -->

