<?xml version="1.0"?>


<!DOCTYPE rdf:RDF [
    <!ENTITY owl "http://www.w3.org/2002/07/owl#" >
    <!ENTITY xsd "http://www.w3.org/2001/XMLSchema#" >
    <!ENTITY rdfs "http://www.w3.org/2000/01/rdf-schema#" >
    <!ENTITY rdf "http://www.w3.org/1999/02/22-rdf-syntax-ns#" >
    <!ENTITY cpannotationschema "http://www.ontologydesignpatterns.org/schemas/cpannotationschema.owl#" >
]>


<rdf:RDF xmlns="http://mklab.iti.gr/pericles/Policy_ODP#"
     xml:base="http://mklab.iti.gr/pericles/Policy_ODP"
     xmlns:rdf="http://www.w3.org/1999/02/22-rdf-syntax-ns#"
     xmlns:owl="http://www.w3.org/2002/07/owl#"
     xmlns:cpannotationschema="http://www.ontologydesignpatterns.org/schemas/cpannotationschema.owl#"
     xmlns:xsd="http://www.w3.org/2001/XMLSchema#"
     xmlns:rdfs="http://www.w3.org/2000/01/rdf-schema#">
    <owl:Ontology rdf:about="http://mklab.iti.gr/pericles/Policy_ODP">
        <cpannotationschema:coversRequirements rdf:datatype="&rdfs;Literal">1. What are the main entities associated with a policy? A policy is usually associated with super/sub-policies, processes, agents and other entities.
2. What are the main attributes of a policy? They are version, language, policy type, requirement level, implementation status and automation status.
3. Where is a policy described? Statements are detailed text (formal or non- formal) definitions of the policy contents.</cpannotationschema:coversRequirements>
        <cpannotationschema:hasIntent>The pattern intends to model policies, their characteristics and their associated entities, such as processes and agents.</cpannotationschema:hasIntent>
        <cpannotationschema:scenarios>Some examples of instantiation of the Policy ODP are:
  1. The policy has two subpolicies
  2. The policy is implemented by a certain process
  3. The policy is validated by a certain process
  4. The policy is assigned to John Smith
  5. The policy is fully automated</cpannotationschema:scenarios>
        <cpannotationschema:hasConsequences>The Policy ODP is expected to facilitate the representation of the policy notion, which can be exploited in various domains. A well-established, comprehensible pattern will prove to be advantageous.</cpannotationschema:hasConsequences>
        <owl:imports rdf:resource="http://www.ontologydesignpatterns.org/schemas/cpannotationschema.owl"/>
        <owl:imports rdf:resource="http://xmlns.com/foaf/0.1/"/>
    </owl:Ontology>
    


    <!-- 
    ///////////////////////////////////////////////////////////////////////////////////////
    //
    // Object Properties
    //
    ///////////////////////////////////////////////////////////////////////////////////////
     -->

    


    <!-- http://mklab.iti.gr/pericles/Policy_ODP#assignedTo -->

    <owl:ObjectProperty rdf:about="http://mklab.iti.gr/pericles/Policy_ODP#assignedTo">
        <rdfs:label>assigned to</rdfs:label>
        <rdfs:comment>Associates a policy to the agent that is responsible for the application of the policy (person or role).</rdfs:comment>
        <rdfs:domain rdf:resource="http://mklab.iti.gr/pericles/Policy_ODP#Policy"/>
        <rdfs:range rdf:resource="http://xmlns.com/foaf/0.1/Agent"/>
    </owl:ObjectProperty>
    


    <!-- http://mklab.iti.gr/pericles/Policy_ODP#hasAutomationStatus -->

    <owl:ObjectProperty rdf:about="http://mklab.iti.gr/pericles/Policy_ODP#hasAutomationStatus">
        <rdfs:label>has automation status</rdfs:label>
        <rdfs:comment>Associates a policy with an automation level.</rdfs:comment>
        <rdfs:range rdf:resource="http://mklab.iti.gr/pericles/Policy_ODP#AutomationStatus"/>
        <rdfs:domain rdf:resource="http://mklab.iti.gr/pericles/Policy_ODP#Policy"/>
    </owl:ObjectProperty>
    


    <!-- http://mklab.iti.gr/pericles/Policy_ODP#hasImplementationStatus -->

    <owl:ObjectProperty rdf:about="http://mklab.iti.gr/pericles/Policy_ODP#hasImplementationStatus">
        <rdfs:label>has implementation status</rdfs:label>
        <rdfs:comment>Associates a policy with an implementation level.</rdfs:comment>
        <rdfs:range rdf:resource="http://mklab.iti.gr/pericles/Policy_ODP#ImplementationStatus"/>
        <rdfs:domain rdf:resource="http://mklab.iti.gr/pericles/Policy_ODP#Policy"/>
    </owl:ObjectProperty>
    


    <!-- http://mklab.iti.gr/pericles/Policy_ODP#hasLanguage -->

    <owl:ObjectProperty rdf:about="http://mklab.iti.gr/pericles/Policy_ODP#hasLanguage">
        <rdfs:label>has language</rdfs:label>
        <rdfs:comment>Associates a policy with the language used for the policy definition.</rdfs:comment>
        <rdfs:range rdf:resource="http://mklab.iti.gr/pericles/Policy_ODP#Language"/>
        <rdfs:domain rdf:resource="http://mklab.iti.gr/pericles/Policy_ODP#Policy"/>
    </owl:ObjectProperty>
    


    <!-- http://mklab.iti.gr/pericles/Policy_ODP#hasPolicyType -->

    <owl:ObjectProperty rdf:about="http://mklab.iti.gr/pericles/Policy_ODP#hasPolicyType">
        <rdfs:label>has policy type</rdfs:label>
        <rdfs:comment>Associates a policy with a policy type.</rdfs:comment>
        <rdfs:domain rdf:resource="http://mklab.iti.gr/pericles/Policy_ODP#Policy"/>
        <rdfs:range rdf:resource="http://mklab.iti.gr/pericles/Policy_ODP#PolicyType"/>
    </owl:ObjectProperty>
    


    <!-- http://mklab.iti.gr/pericles/Policy_ODP#hasRequirementLevel -->

    <owl:ObjectProperty rdf:about="http://mklab.iti.gr/pericles/Policy_ODP#hasRequirementLevel">
        <rdfs:label>has requirement level</rdfs:label>
        <rdfs:comment>Associates a policy with an requirement level.</rdfs:comment>
        <rdfs:domain rdf:resource="http://mklab.iti.gr/pericles/Policy_ODP#Policy"/>
        <rdfs:range rdf:resource="http://mklab.iti.gr/pericles/Policy_ODP#RequirementLevel"/>
    </owl:ObjectProperty>
    


    <!-- http://mklab.iti.gr/pericles/Policy_ODP#hasStatement -->

    <owl:ObjectProperty rdf:about="http://mklab.iti.gr/pericles/Policy_ODP#hasStatement">
        <rdfs:label>has statement</rdfs:label>
        <rdfs:comment>Associates a policy with a statement, which is a detailed definition of the policy contents.</rdfs:comment>
        <rdfs:domain rdf:resource="http://mklab.iti.gr/pericles/Policy_ODP#Policy"/>
        <rdfs:range rdf:resource="http://mklab.iti.gr/pericles/Policy_ODP#Statement"/>
    </owl:ObjectProperty>
    


    <!-- http://mklab.iti.gr/pericles/Policy_ODP#hasSubPolicy -->

    <owl:ObjectProperty rdf:about="http://mklab.iti.gr/pericles/Policy_ODP#hasSubPolicy">
        <rdfs:label>has subpolicy</rdfs:label>
        <rdfs:comment>Associates a policy to another policy that is contained in the initial.</rdfs:comment>
        <rdfs:domain rdf:resource="http://mklab.iti.gr/pericles/Policy_ODP#Policy"/>
        <rdfs:range rdf:resource="http://mklab.iti.gr/pericles/Policy_ODP#Policy"/>
    </owl:ObjectProperty>
    


    <!-- http://mklab.iti.gr/pericles/Policy_ODP#hasValidationProcess -->

    <owl:ObjectProperty rdf:about="http://mklab.iti.gr/pericles/Policy_ODP#hasValidationProcess">
        <rdfs:label>has validation process</rdfs:label>
        <rdfs:comment>Associates a policy with a process that is used to validate the policy.</rdfs:comment>
        <rdfs:domain rdf:resource="http://mklab.iti.gr/pericles/Policy_ODP#Policy"/>
        <rdfs:range rdf:resource="http://mklab.iti.gr/pericles/Policy_ODP#Process"/>
    </owl:ObjectProperty>
    


    <!-- http://mklab.iti.gr/pericles/Policy_ODP#hasVersion -->

    <owl:ObjectProperty rdf:about="http://mklab.iti.gr/pericles/Policy_ODP#hasVersion">
        <rdfs:label>has version</rdfs:label>
        <rdfs:comment>Defines a policy&apos;s version.</rdfs:comment>
        <rdfs:range rdf:resource="http://mklab.iti.gr/pericles/Policy_ODP#Version"/>
    </owl:ObjectProperty>
    


    <!-- http://mklab.iti.gr/pericles/Policy_ODP#implementedBy -->

    <owl:ObjectProperty rdf:about="http://mklab.iti.gr/pericles/Policy_ODP#implementedBy">
        <rdfs:label>implemented by</rdfs:label>
        <rdfs:comment>Associates a policy with a process that is used to implement the policy.</rdfs:comment>
        <rdfs:domain rdf:resource="http://mklab.iti.gr/pericles/Policy_ODP#Policy"/>
        <rdfs:range rdf:resource="http://mklab.iti.gr/pericles/Policy_ODP#Process"/>
    </owl:ObjectProperty>
    


    <!-- http://mklab.iti.gr/pericles/Policy_ODP#targetsEntity -->

    <owl:ObjectProperty rdf:about="http://mklab.iti.gr/pericles/Policy_ODP#targetsEntity">
        <rdfs:label>targets entity</rdfs:label>
        <rdfs:comment>Associates a policy with an entity that is subject to the policy.</rdfs:comment>
        <rdfs:domain rdf:resource="http://mklab.iti.gr/pericles/Policy_ODP#Policy"/>
        <rdfs:range rdf:resource="&owl;Thing"/>
    </owl:ObjectProperty>
    


    <!-- http://mklab.iti.gr/pericles/Policy_ODP#targetsUsers -->

    <owl:ObjectProperty rdf:about="http://mklab.iti.gr/pericles/Policy_ODP#targetsUsers">
        <rdfs:label>targets users</rdfs:label>
        <rdfs:comment>Associates a policy to the user community the policy has been designed for.</rdfs:comment>
        <rdfs:domain rdf:resource="http://mklab.iti.gr/pericles/Policy_ODP#Policy"/>
        <rdfs:range rdf:resource="http://xmlns.com/foaf/0.1/Group"/>
    </owl:ObjectProperty>
    


    <!-- 
    ///////////////////////////////////////////////////////////////////////////////////////
    //
    // Classes
    //
    ///////////////////////////////////////////////////////////////////////////////////////
     -->

    


    <!-- http://mklab.iti.gr/pericles/Policy_ODP#AutomationStatus -->

    <owl:Class rdf:about="http://mklab.iti.gr/pericles/Policy_ODP#AutomationStatus">
        <rdfs:label>Automation Status</rdfs:label>
        <rdfs:subClassOf rdf:resource="http://mklab.iti.gr/pericles/Policy_ODP#Descriptor"/>
        <rdfs:comment>The level of automation of a policy. Specifies if a policy implementation requires human intervention.</rdfs:comment>
        <rdfs:comment>E.g. manual, automated with human intervention, automated with human validation, fully automated, etc.</rdfs:comment>
    </owl:Class>
    


    <!-- http://mklab.iti.gr/pericles/Policy_ODP#Descriptor -->

    <owl:Class rdf:about="http://mklab.iti.gr/pericles/Policy_ODP#Descriptor">
        <rdfs:label>Descriptor</rdfs:label>
        <rdfs:comment>The various elements describing a policy.</rdfs:comment>
    </owl:Class>
    


    <!-- http://mklab.iti.gr/pericles/Policy_ODP#ImplementationStatus -->

    <owl:Class rdf:about="http://mklab.iti.gr/pericles/Policy_ODP#ImplementationStatus">
        <rdfs:label>Implementation Status</rdfs:label>
        <rdfs:subClassOf rdf:resource="http://mklab.iti.gr/pericles/Policy_ODP#Descriptor"/>
        <rdfs:comment>E.g. implemented, partially implemented, unimplemented, not-implementable, etc.</rdfs:comment>
        <rdfs:comment>The level of implementation of a policy</rdfs:comment>
    </owl:Class>
    


    <!-- http://mklab.iti.gr/pericles/Policy_ODP#Language -->

    <owl:Class rdf:about="http://mklab.iti.gr/pericles/Policy_ODP#Language">
        <rdfs:label>Language</rdfs:label>
        <rdfs:subClassOf rdf:resource="http://mklab.iti.gr/pericles/Policy_ODP#Descriptor"/>
        <rdfs:comment>The language used for the policy definition</rdfs:comment>
        <rdfs:comment>E.g. natural language, ReAL, SPIN, etc.</rdfs:comment>
    </owl:Class>
    


    <!-- http://mklab.iti.gr/pericles/Policy_ODP#Policy -->

    <owl:Class rdf:about="http://mklab.iti.gr/pericles/Policy_ODP#Policy">
        <rdfs:label>Policy</rdfs:label>
        <rdfs:comment>A deliberate system of principles to guide decisions and achieve rational outcomes. A policy is a statement of intent, and is implemented as a procedure or protocol.</rdfs:comment>
    </owl:Class>
    


    <!-- http://mklab.iti.gr/pericles/Policy_ODP#PolicyType -->

    <owl:Class rdf:about="http://mklab.iti.gr/pericles/Policy_ODP#PolicyType">
        <rdfs:label>Policy Type</rdfs:label>
        <rdfs:subClassOf rdf:resource="http://mklab.iti.gr/pericles/Policy_ODP#Descriptor"/>
        <rdfs:comment>The type of policy.</rdfs:comment>
        <rdfs:comment>Not all policies are equal; mandatory ones must be implemented to satisfy law or other requirements, others are aspirational, and most are met with the best possible effort.</rdfs:comment>
        <rdfs:comment>E.g. mandatory, legal requirement, aspirational, business driven, etc.</rdfs:comment>
    </owl:Class>
    


    <!-- http://mklab.iti.gr/pericles/Policy_ODP#Process -->

    <owl:Class rdf:about="http://mklab.iti.gr/pericles/Policy_ODP#Process">
        <rdfs:label>Process</rdfs:label>
        <rdfs:subClassOf rdf:resource="&owl;Thing"/>
        <rdfs:comment>A sequence of interdependent and linked procedures which, at every stage, consume one or more resources (time, energy, machines, money) to convert inputs (data, material, parts, etc.) into outputs.</rdfs:comment>
    </owl:Class>
    


    <!-- http://mklab.iti.gr/pericles/Policy_ODP#RequirementLevel -->

    <owl:Class rdf:about="http://mklab.iti.gr/pericles/Policy_ODP#RequirementLevel">
        <rdfs:label>Requirement Level</rdfs:label>
        <rdfs:subClassOf rdf:resource="http://mklab.iti.gr/pericles/Policy_ODP#Descriptor"/>
        <rdfs:comment>E.g. must, must not, should, shoud not, may, etc.</rdfs:comment>
        <rdfs:comment>The level of a policy&apos;s compliance</rdfs:comment>
    </owl:Class>
    


    <!-- http://mklab.iti.gr/pericles/Policy_ODP#Statement -->

    <owl:Class rdf:about="http://mklab.iti.gr/pericles/Policy_ODP#Statement">
        <rdfs:label>Statement</rdfs:label>
        <rdfs:subClassOf rdf:resource="http://mklab.iti.gr/pericles/Policy_ODP#Descriptor"/>
        <rdfs:comment>Detailed definition of the policy contents.</rdfs:comment>
    </owl:Class>
    


    <!-- http://mklab.iti.gr/pericles/Policy_ODP#Version -->

    <owl:Class rdf:about="http://mklab.iti.gr/pericles/Policy_ODP#Version">
        <rdfs:label>Version</rdfs:label>
        <rdfs:subClassOf rdf:resource="http://mklab.iti.gr/pericles/Policy_ODP#Descriptor"/>
        <rdfs:comment>A policy&apos;s version</rdfs:comment>
    </owl:Class>
</rdf:RDF>



<!-- Generated by the OWL API (version 3.5.1) http://owlapi.sourceforge.net -->

